# baseURI: http://www.enridaga.net/datavok/edit
# imports: file:/Users/enricox/Dropbox/PhD/WEBIST2014/survey/step-3/draft-vok-defs.nt
# imports: file:/Users/enricox/Dropbox/PhD/WEBIST2014/survey/step-3/draft-vok-subs.nt
# imports: http://xmlns.com/foaf/spec/

@prefix :        <http://www.enridaga.net/datavok/edit#> .
@prefix dvok:    <http://www.enridaga.net/datavok/draft#> .
@prefix evok:    <http://www.enridaga.net/datavok/edit#> .
@prefix foaf:    <http://xmlns.com/foaf/0.1/> .
@prefix owl:     <http://www.w3.org/2002/07/owl#> .
@prefix rdf:     <http://www.w3.org/1999/02/22-rdf-syntax-ns#> .
@prefix rdfs:    <http://www.w3.org/2000/01/rdf-schema#> .
@prefix vs:      <http://www.w3.org/2003/06/sw-vocab-status/ns#> .
@prefix xsd:     <http://www.w3.org/2001/XMLSchema#> .

dvok:Clean
      rdfs:subClassOf dvok:Task .

dvok:Cluster
      rdfs:subClassOf evok:Operation .

dvok:Collect
      rdfs:subClassOf evok:Operation .

dvok:Compare
      rdfs:subClassOf evok:Operation .

dvok:Compute
      rdfs:subClassOf evok:Operation .

dvok:Concat
      rdfs:subClassOf evok:Operation .

dvok:Consider
      rdfs:subClassOf evok:Operation .

dvok:Create
      rdfs:subClassOf evok:Operation .

dvok:Delete
      rdfs:subClassOf evok:Operation .

dvok:Describe
      rdfs:subClassOf evok:Operation .

dvok:Description
      rdfs:subClassOf dvok:Data .

dvok:Detect
      rdfs:subClassOf evok:Operation .

dvok:Discover
      rdfs:subClassOf dvok:Task .

dvok:Entity
      rdfs:comment "At one point we need to decouple the URI (Pointer?) from the Thing (Entity)"^^xsd:string .

dvok:Explain
      rdfs:subClassOf dvok:Task .

dvok:Extract
      rdfs:subClassOf evok:Operation .

dvok:Identify
      rdfs:subClassOf evok:Operation .

dvok:Lift
      rdfs:subClassOf evok:Operation .

dvok:Link
      rdfs:subClassOf evok:Operation .

dvok:Listen
      rdfs:subClassOf evok:Operation .

dvok:Map
      rdfs:subClassOf evok:Operation .

dvok:NamedDataset
      rdfs:subClassOf dvok:Dataset .

dvok:Ontology
      rdfs:subClassOf dvok:Vocabulary .

dvok:Optimize
      rdfs:subClassOf dvok:Task .

dvok:Photograph
      rdfs:subClassOf evok:Operation .

dvok:Pointer
      rdfs:comment "See also Entity. This should refer to Identifiers (URIs in RDF triples). Which is not the same as Locator (only a subset of the identifiers are locators...)"^^xsd:string .

dvok:Preserve
      rdfs:subClassOf evok:Operation .

dvok:Provider
      rdfs:subClassOf foaf:Agent .

dvok:Rank
      rdfs:subClassOf evok:Operation .

dvok:Stand-In
      rdfs:subClassOf dvok:Data .

dvok:Summarize
      rdfs:subClassOf dvok:Task .

dvok:Truncate
      rdfs:subClassOf dvok:Collect .

dvok:Vocabulary
      rdfs:subClassOf dvok:Descriptor .

dvok:about
      rdfs:subPropertyOf dvok:linked-to .

dvok:affects
      rdfs:subPropertyOf dvok:linked-to .

dvok:annotated-by
      rdfs:domain dvok:Data .

dvok:annotation
      rdfs:comment "the term anotation is misleading here"^^xsd:string ;
      rdfs:subPropertyOf dvok:extracted-from .

dvok:attached-to
      rdfs:subPropertyOf dvok:linked-to .

dvok:before
      rdfs:subPropertyOf evok:version-of .

dvok:combination-from
      rdfs:subPropertyOf evok:derive-from .

dvok:compared-with
      rdfs:subPropertyOf dvok:linked-to .

dvok:component-of
      rdfs:subPropertyOf dvok:linked-to .

dvok:current-version-of
      rdfs:subPropertyOf evok:version-of .

dvok:distinct-set
      rdfs:subPropertyOf dvok:part-of .

dvok:duplicate-of
      rdfs:subPropertyOf dvok:compared-with .

dvok:extract
      rdfs:comment "This is not a property"^^xsd:string .

dvok:extracted-from
      rdfs:subPropertyOf evok:derive-from .

dvok:in-tuple-with
      rdfs:subPropertyOf dvok:linked-to .

dvok:inferred-from
      rdfs:subPropertyOf evok:derive-from .

dvok:known-data
      rdfs:comment "This is probably not a property"^^xsd:string .

dvok:linked-to
      rdfs:domain dvok:Data ;
      rdfs:range dvok:Data .

dvok:lost-part-of
      rdfs:comment "It looks like here the comment is not inline with the sentence. What does \"lost\" means here? 1. a wrong property name 8same as meaningless) or 2. the relation between some data and some other data which is the one from the first is derived by mean of a method wich makes some data not anymore identifiable."^^xsd:string .

dvok:message
      rdfs:comment "Well this should probably be refactored to the Class Message"^^xsd:string .

dvok:newer-version-of
      rdfs:subPropertyOf evok:version-of ;
      owl:inverseOf dvok:before .

dvok:not-fits
      owl:inverseOf dvok:fits .

dvok:related-to
      rdfs:comment "Unsure if this is a kind of linked-to or a relation between Data and Concern"^^xsd:string .

dvok:sample-of
      rdfs:subPropertyOf evok:derive-from , dvok:part-of .

dvok:shares-capability-with
      rdfs:subPropertyOf dvok:compared-with .

dvok:similar-to
      rdfs:subPropertyOf dvok:compared-with .

dvok:snapshot-of
      rdfs:subPropertyOf evok:version-of .

dvok:stand-in-of
      rdfs:domain dvok:Stand-In ;
      rdfs:subPropertyOf evok:derive-from .

dvok:sum-of
      rdfs:subPropertyOf dvok:inferred-from .

dvok:summarization-of
      rdfs:subPropertyOf evok:derive-from .

dvok:takes-the-role-of
      rdfs:subPropertyOf evok:same-role-as .

dvok:textual-component-of
      rdfs:subPropertyOf dvok:component-of .

dvok:update-of
      rdfs:comment "Being an update does not necessarily imply being a version. Think about incremental updates, which is the part of the next version of... (considering an upate as an add-only process)"^^xsd:string ;
      rdfs:subPropertyOf dvok:linked-to .

<http://www.enridaga.net/datavok/edit>
      rdf:type owl:Ontology ;
      owl:imports <http://xmlns.com/foaf/spec/> , <file:./draft-vok-defs.nt> , <file:./draft-vok-subs.nt> ;
      owl:versionInfo "Created with TopBraid Composer"^^xsd:string .

evok:Operation
      rdf:type rdfs:Class ;
      rdfs:comment "Operation is not Operator"^^xsd:string ;
      vs:term_status "Proposal"^^xsd:string .

evok:derive-from
      rdf:type rdf:Property ;
      rdfs:subPropertyOf dvok:linked-to .

evok:same-role-as
      rdf:type rdf:Property ;
      rdfs:subPropertyOf dvok:linked-to .

evok:version-of
      rdf:type rdf:Property ;
      rdfs:subPropertyOf dvok:linked-to ;
      vs:term_status ""^^xsd:string .

rdf:Property
      rdf:type rdfs:Class ;
      rdfs:subClassOf dvok:Descriptor ;
      vs:term_status ""^^xsd:string .

rdfs:Class
      rdfs:subClassOf dvok:Descriptor .
